Bdd/Unused.lean
@@ -4,7 +4,7 @@ import all Bdd.Basic
 import all Bdd.Size
 
 section not_used
-open Pointer
+open Pointer Bdd
 
 inductive Pointer.le {m} : Pointer m → Pointer m → Prop where
   | terminal_le_terminal {b c} : b ≤ c → le (terminal b) (terminal c)
@@ -132,9 +132,9 @@ def Pointer.decidableEitherReachable {n m} (O U : OBdd n m) (h : O.1.heap = U.1.
     DecidablePred (fun q ↦ (Reachable O.1.heap O.1.root q) ∨ (Reachable O.1.heap U.1.root q)) := by
   intro p
   simp
-  cases instDecidableReachable O p with
+  cases OBdd.instDecidableReachable O p with
   | isFalse hf =>
-    cases instDecidableReachable U p with
+    cases OBdd.instDecidableReachable U p with
     | isFalse hhf =>
       apply isFalse
       simp_all [or_self, not_false_eq_true]
@@ -196,6 +196,101 @@ instance Bdd.instDecidableEqRelevantPointer : DecidableEq (Bdd.RelevantPointer B
 instance OBdd.instReducedDecidable {n m} : DecidablePred (α := OBdd n m) Reduced :=
   fun _ ↦ (instDecidableAnd (dp := Fintype.decidableForallFintype) (dq := Fintype.decidableForallFintype))
 
+/-- An acyclicity lemma: an edge from `O` to `U` implies that `O` is not reachable from `U`.  -/
+lemma OBdd.not_oedge_reachable {n m} {O U : OBdd n m}: OEdge O U → ¬ Reachable O.1.heap U.1.root O.1.root := by
+  rintro ⟨same_heap, e⟩ contra
+  apply Relation.reflTransGen_iff_eq_or_transGen.mp at contra
+  cases contra with
+  | inl h =>
+    rw [← h] at e
+    exact Bdd.no_self_edge_of_ordered O.ordered O.bdd.relevant_root e
+  | inr h =>
+    apply Relation.TransGen.head'_iff.mp at h
+    rcases h with ⟨c, h1, h2⟩
+    rw [same_heap] at h1
+    let V : OBdd n m := ⟨{heap := U.1.heap, root := c}, ordered_of_edge U.ordered h1⟩
+    have : c = V.1.root := rfl
+    rw [this] at h1 h2
+    apply not_oedge_reachable ⟨by rfl, h1⟩
+    trans O.1.root
+    rw [same_heap] at h2; exact h2
+    rw [← same_heap]; exact Reachable.ofEdge e
+termination_by O
+
+lemma OBdd.eq_root_disjoint_reachable_low_or_high {O : OBdd n m} (h : O.1.root = node j) :
+    Disjoint
+      (· = O.1.root)
+      (fun p ↦ (Reachable O.1.heap (O.low  h).1.root p ∨ Reachable O.1.heap (O.high h).1.root p)) := by
+  intro P h1 h2 p hp
+  specialize h1 p hp
+  specialize h2 p hp
+  simp_all only
+  cases h2 with
+  | inl l =>
+    rw [← h] at l
+    apply OBdd.not_oedge_reachable oedge_of_low l
+  | inr l =>
+    rw [← h] at l
+    apply OBdd.not_oedge_reachable oedge_of_high l
+
+/-- The `Edge` relation lifted to `RelevantPointer`s. -/
+@[simp]
+abbrev Bdd.RelevantEdge {n m} (B : Bdd n m) (p q : B.RelevantPointer) :=
+  Edge B.heap p.1 q.1
+
+lemma Bdd.relevantEdge_of_edge_of_reachable {n m}  {B : Bdd n m} {p q}
+    (e : Edge B.heap p q) (hp : Reachable B.heap B.root p) :
+  RelevantEdge B ⟨p, hp⟩ ⟨q, .snoc hp e⟩ := e
+
+@[simp]
+def RelevantPointer.var {n m} {B : Bdd n m} (p : B.RelevantPointer) : Nat := p.1.toVar B.heap
+
+@[simp]
+def RelevantPointer.gap {n m} {B : Bdd n m} (p : B.RelevantPointer) : Nat := n - (RelevantPointer.var p)
+
+theorem RelevantEdge.flip_wellFounded (o : Ordered B) : WellFounded (flip (RelevantEdge B)) := by
+  have : Subrelation (flip (RelevantEdge B)) (InvImage Nat.lt RelevantPointer.gap) := by
+    rintro ⟨x, hx⟩ ⟨y, hy⟩ e
+    simp_all only [InvImage, flip, RelevantPointer.gap]
+    apply Nat.sub_lt_sub_left
+    cases e <;> simp
+    simp [B.ordered_iff'.1 o y x hy e]
+  exact Subrelation.wf this (InvImage.wf _ (Nat.lt_wfRel.wf))
+
+instance RelevantEdge.instWellFoundedRelation {n m} (O : OBdd n m) : WellFoundedRelation O.1.RelevantPointer where
+  rel := flip O.1.RelevantEdge
+  wf  := (RelevantEdge.flip_wellFounded O.2)
+
+lemma OBdd.reachable_from_node_iff' {n m j p} {O : OBdd n m} (h : O.1.root = node j) :
+    Reachable O.1.heap O.1.root p ↔ p = O.1.root ∨ (Reachable O.1.heap (O.low h).1.root p ∨ Reachable O.1.heap (O.high h).1.root p) := by
+  constructor
+  · intro r
+    cases r with
+    | refl => left; rfl
+    | cons e r =>
+      rename_i q
+      right
+      rw [h] at e
+      cases e with
+      | low =>
+        left
+        rw [low_root_eq_low]
+        exact r
+      | high =>
+        right
+        rw [high_root_eq_high]
+        exact r
+  · intro r
+    cases r with
+    | inl r =>
+      rw [r]
+      left
+    | inr r =>
+      simp only [low_root_eq_low, high_root_eq_high] at r
+      cases r with
+      | inl r => exact .trans (O.bdd.reachable_low h) r
+      | inr r => exact .trans (O.bdd.reachable_high h) r
+
 lemma OBdd.card_reachable_node' {O : OBdd n m} (h : O.1.root = node j) :
   Fintype.card {p // Reachable O.1.heap O.1.root p} =
   Fintype.card {p // p = O.1.root ∨ (Reachable O.1.heap (O.low  h).1.root p ∨ Reachable O.1.heap (O.high h).1.root p)} := by
@@ -243,7 +338,197 @@ decreasing_by
   · exact Edge.high
   · exact Edge.low
 
+def OBdd.isTerminal {n m} (O : OBdd n m) := ∃ b, O.1.root = terminal b
+
+lemma not_OEdge_of_isTerminal {O : OBdd n m}: O.isTerminal → ¬ OEdge O U := by
+  rintro ⟨b, h⟩ ⟨_, contra⟩
+  rw [h] at contra
+  exact not_terminal_edge contra
+
+lemma not_isTerminal_of_root_eq_node {n m} {j} {O : OBdd n m} (h : O.1.root = node j) : ¬ O.isTerminal := by
+  rintro ⟨b, hb⟩
+  rw [h] at hb
+  contradiction
+
+lemma Bdd.terminal_of_zero_vars {B : Bdd n m} : n = 0 → ∃ b, B.root = .terminal b := by
+  intro h
+  subst h
+  cases hr : B.root with
+  | terminal b => exact ⟨b, rfl⟩
+  | node j => exact False.elim (Nat.not_lt_zero _ B.heap[j].var.2)
+
+lemma Bdd.terminal_of_zero_heap {B : Bdd n m} : m = 0 → ∃ b, B.root = .terminal b := by
+  intro h
+  subst h
+  cases hr : B.root with
+  | terminal b => exact ⟨b, rfl⟩
+  | node j => exact False.elim (Nat.not_lt_zero _ j.2)
+
+/-- The `OEdge` relation between Ordered BDDs is well-founded. -/
+theorem OEdge.wellFounded {n m} : @WellFounded (OBdd n m) OEdge := by
+  suffices s : Subrelation (@OEdge n m) (InvImage Nat.lt (OBdd.var ·)) from
+    Subrelation.wf s (InvImage.wf _ (Nat.lt_wfRel.wf))
+  rintro ⟨x, hx⟩ ⟨y, hy⟩ ⟨h1, h2⟩
+  simp_all only
+  simp only [InvImage, OBdd.var, Nat.lt_eq, Fin.val_fin_lt, var]
+  simp only [ordered_iff'] at hx
+  rw [← h1] at h2 ⊢
+  exact hx x.root y.root .refl h2
+
+/-- The only reduced BDD that denotes a constant function is the terminal BDD. -/
+theorem OBdd.terminal_of_constant (O : OBdd n m) :
+    O.Reduced → O.evaluate = (fun _ ↦ b) → O.1.root = terminal b := by
+  intro R h
+  cases O_root_def : O.1.root
+  case terminal b' =>
+    grind only [OBdd.evaluate_terminal O_root_def]
+  case node j =>
+    exfalso
+    refine not_reduced_of_sim_high_low O_root_def ?_ R
+    have : (O.high O_root_def).evaluate = (O.low O_root_def).evaluate := by
+      ext I
+      trans b
+      · simp [evaluate_high_eq_evaluate_set_true, h]
+      · simp [evaluate_low_eq_evaluate_set_false, h]
+    exact OBdd.Canonicity (high_reduced R) (low_reduced R) this
+
+lemma OBdd.reduced_var_dependent {n m} {O : OBdd n m} {p : Fin n} :
+    O.Reduced → (∀ i : Fin p, Nary.IndependentOf (O.evaluate) ⟨i.1, by omega⟩) → p.1 ≤ O.1.var.1 := by
+  intro hr hp
+  cases O_root_def : O.1.root with
+  | terminal _ =>
+    simp only [Nat.succ_eq_add_one, Bdd.var, O_root_def, Pointer.toVar_terminal]
+    exact Fin.le_last p.castSucc
+  | node j =>
+    by_contra c
+    simp only [not_le] at c
+    have := hp ⟨O.1.var, by aesop⟩
+    simp only [Nat.succ_eq_add_one] at this
+    suffices s : (O.high O_root_def).evaluate = (O.low O_root_def).evaluate by
+      absurd hr
+      apply not_reduced_of_sim_high_low O_root_def
+      apply OBdd.Canonicity (OBdd.high_reduced hr) (OBdd.low_reduced hr) s
+    ext I
+    trans O.evaluate I
+    · simp only [Bdd.var, O_root_def, Pointer.toVar_node, Fin.eta] at this
+      have := this true I
+      rw [this]
+      rw [OBdd.evaluate_node' O_root_def]
+      simp only [Fin.getElem_fin, Vector.getElem_set_self]
+      simp only [↓reduceIte]
+      suffices s : Nary.IndependentOf (O.high O_root_def).evaluate O.1.heap[j.1].var by rw [← s true I]
+      refine independentOf_lt_root (O.high O_root_def) ⟨O.1.heap[j.1].var.1, ?_⟩
+      convert OBdd.var_lt_high_var
+      simp only [O.var_node O_root_def, Fin.getElem_fin]
+    · symm
+      simp only [Bdd.var, O_root_def, Pointer.toVar_node, Fin.eta] at this
+      have := this false I
+      rw [this]
+      rw [OBdd.evaluate_node' O_root_def]
+      simp only [Fin.getElem_fin, Vector.getElem_set_self]
+      simp only [Bool.false_eq_true, ↓reduceIte]
+      suffices s : Nary.IndependentOf (O.low O_root_def).evaluate O.1.heap[j.1].var by rw [s false I]
+      refine independentOf_lt_root (O.low O_root_def) ⟨O.1.heap[j.1].var.1, ?_⟩
+      convert OBdd.var_lt_low_var
+      simp only [O.var_node O_root_def, Fin.getElem_fin]
+
+lemma Bdd.ordered_of_ordered_heap_not_reachable_set (O : OBdd n m) :
+    ∀ i N, ¬ Reachable O.1.heap O.1.root (node i) → Ordered ⟨O.1.heap.set i N, O.1.root⟩ := by
+  intro i N unr
+  induction O using OBdd.init_inductionOn with
+  | base b O' h1 h2 => exact ordered_of_terminal h2
+  | step O' j h1 h2 ih_low ih_high =>
+    have h3 : i ≠ j := by
+      intro contra
+      rw [contra] at unr
+      rw [h2] at unr
+      apply unr
+      left
+    apply ordered_of_low_high_ordered (by rw [h2])
+    · simp only [low, Fin.getElem_fin]
+      rw [Vector.getElem_set_ne i.2 j.2 (Fin.val_ne_of_ne h3)]
+      apply ih_low
+      intro h4
+      apply unr
+      trans O'.1.heap[j].low
+      · exact O'.bdd.reachable_low h2
+      · exact h4
+    · simp only [var_eq, low, Fin.getElem_fin]
+      rw [Vector.getElem_set_ne i.2 j.2 (Fin.val_ne_of_ne h3)]
+      rw [h2, toVar_heap_set h3]
+      have h4 : toVar O'.1.heap (node j) < toVar O'.1.heap O'.1.heap[j].low :=
+        ordered_iff'.1 O'.ordered (node j) O'.1.heap[j].low (h2 ▸ .refl) Edge.low
+      convert h4 using 1
+      cases low_def : O.1.heap[j].low with
+      | terminal bl =>
+        simp_all only [Fin.getElem_fin, toVar_terminal]
+      | node jl =>
+        simp only [← h1, Fin.getElem_fin] at low_def
+        simp only [low_def, Fin.getElem_fin]
+        simp only [Fin.ext_iff, toVar_node, Fin.getElem_fin]
+        rw [Vector.getElem_set_ne i.2 jl.2]
+        simp only [ne_eq, Fin.val_inj]
+        intro rfl
+        apply unr
+        rw [← low_def]
+        exact O'.bdd.reachable_low h2
+    · simp only [high, Fin.getElem_fin]
+      rw [Vector.getElem_set_ne i.2 j.2 (Fin.val_ne_of_ne h3)]
+      apply ih_high
+      intro h4
+      apply unr
+      trans O'.1.heap[j].high
+      · exact O'.bdd.reachable_high h2
+      · exact h4
+    · simp only [var_eq, high, Fin.getElem_fin]
+      rw [Vector.getElem_set_ne i.2 j.2 (Fin.val_ne_of_ne h3)]
+      rw [h2, toVar_heap_set h3]
+      have h4 : toVar O'.1.heap (node j) < toVar O'.1.heap O'.1.heap[j].high :=
+        ordered_iff'.1 O'.ordered (node j) O'.1.heap[j].high (h2 ▸ .refl) Edge.high
+      convert h4 using 1
+      cases high_def : O.1.heap[j].high with
+      | terminal bl =>
+        simp_all only [Fin.getElem_fin, toVar_terminal]
+      | node jl =>
+        simp only [← h1, Fin.getElem_fin] at high_def
+        simp only [high_def, Fin.getElem_fin]
+        simp only [Fin.ext_iff, toVar_node, Fin.getElem_fin]
+        rw [Vector.getElem_set_ne i.2 jl.2]
+        simp only [ne_eq, Fin.val_inj]
+        intro rfl
+        apply unr
+        rw [← high_def]
+        exact O'.bdd.reachable_high h2
+
+lemma OBdd.ordered_of_edge {n m} {O : OBdd n m} (p : Pointer m) :
+    Edge O.bdd.heap O.bdd.root p → Bdd.Ordered {heap := O.bdd.heap, root := p} := by
+  intro e
+  exact ordered_of_relevant O ⟨p, Reachable.ofEdge e⟩
+
+lemma OBdd.evaluate_eq_of_forall_usesVar {O : OBdd n m} {I J : Vector Bool n} :
+    (∀ i, O.1.usesVar i → I[i] = J[i]) → O.evaluate I = O.evaluate J := by
+  intro h
+  apply Nary.eq_of_forall_dependency_getElem_eq
+  rintro ⟨i, hi⟩
+  apply h
+  simp only [Nary.DependsOn, Nary.IndependentOf, not_forall] at hi
+  rcases hi with ⟨b, v, hbv⟩
+  apply usesVar_of_dependsOn hbv
+
 namespace Size
+
+lemma isTerminal_iff_size_eq_zero {n m} {O : OBdd n m} : size O = 0 ↔ O.isTerminal := by
+  constructor
+  · intro h
+    simp only [size, Function.comp_apply, List.length_eq_zero_iff] at h
+    cases O_root_def : O.1.root with
+    | terminal b => use b
+    | node j =>
+      have := Collect.collect_spec (j := j) (by rw [O_root_def]; exact Pointer.Reachable.refl)
+      rw [h] at this
+      contradiction
+  · rintro ⟨b, hb⟩
+    simp [size, Collect.collect_terminal hb]
 
 def bool_of_size_eq_zero {n m} (O : OBdd n m) (h : size O = 0) : Bool :=
   match O_root_def : O.1.root with
